wip --- updating varsets to ssr

examples/ghc/theories/Var.v
@@ -1,3 +1,5 @@
+From Coq Require Import ssreflect ssrfun ssrbool.
+
 Require Import Id.
 Require Import Core. (* For [Var] only *)
 Require Import Unique.
@@ -5,13 +7,13 @@ Require Import Unique.
 Require Import Coq.Structures.Equalities.
 
 Require Import GHC.Base.
-Import GHC.Base.ManualNotations.
 
 Require Import Proofs.GHC.Base.
 Require Import Proofs.Data.Foldable.
 Require Import Proofs.Data.Traversable.
 Require Import Proofs.Unique.
 
+(*
 Ltac unfold_zeze :=
   unfold GHC.Base.op_zeze__, Core.Eq___Var, op_zeze____, 
   Core.Eq___Var_op_zeze__, Eq_Char___;
@@ -20,7 +22,12 @@ Ltac unfold_zsze :=
   unfold GHC.Base.op_zsze__, Core.Eq___Var, op_zsze____, 
   Core.Eq___Var_op_zsze__, Eq_Char___;
   unfold GHC.Base.op_zsze__, Nat.Eq_nat, op_zsze____.  
+*)
 
+Ltac unfold_zeze := 
+  repeat (GHC.Base.unfold_zeze; unfold Core.Eq___Var, Core.Eq___Var_op_zeze__).
+Ltac unfold_zsze :=
+  repeat (GHC.Base.unfold_zsze; unfold Core.Eq___Var, Core.Eq___Var_op_zsze__).
 
 (** ** Stuff about [Var] and [Unique] *)
 
@@ -37,7 +44,7 @@ Qed.
 
 (* Equal vars have equal keys *)
 Lemma eq_unique : forall (v1 v2: Var), 
-    (v1 == v2) = true <->
+    (v1 == v2) <->
     Unique.getWordKey (Unique.getUnique v1) = 
     Unique.getWordKey (Unique.getUnique v2). 
 Proof.
@@ -49,49 +56,6 @@ Proof.
   destruct v1; destruct v2; simpl;
   apply N.eqb_eq.
 Qed.
-
-(** ** [varUnique] *)
-
-
-Lemma varUnique_iff :
-  forall v1 v2,
-    v1 == v2 = true <-> varUnique v1 = varUnique v2.
-Proof.
-  intros.
-  unfold_zeze.
-  unfold varUnique.
-  set (n1 := realUnique v1).
-  set (n2 := realUnique v2).
-  rewrite N.eqb_eq.
-  unfold Unique.mkUniqueGrimily in *.
-  intuition congruence.
-Qed.
-
-
-Lemma In_varUnique_elem : forall a l, 
-    In (varUnique a) (map varUnique l) <-> 
-    Foldable.elem a l = true.
-Proof.
-  intros.
-  induction l.
-  - simpl. rewrite elem_nil.
-    split; intro. contradiction. discriminate.
-  - rewrite elem_cons.
-    rewrite orb_true_iff.
-    split.
-    intro h. inversion h.
-    left. 
-    rewrite varUnique_iff in *.
-    auto.
-    right. tauto.
-    intro h.
-    rewrite <- IHl in h.
-    simpl.
-    destruct h.
-    left. rewrite varUnique_iff in *. auto.
-    right. auto.
-Qed.
-
 
 Instance EqLaws_Var : EqLaws Var := {}.
 Proof.
@@ -115,6 +79,56 @@ Proof.
     reflexivity.
 Qed.
 
+
+(** ** [varUnique] *)
+
+
+Lemma varUnique_iff :
+  forall v1 v2,
+    v1 == v2 <-> varUnique v1 = varUnique v2.
+Proof.
+  intros.
+  unfold_zeze.
+  unfold varUnique.
+  set (n1 := realUnique v1).
+  set (n2 := realUnique v2).
+  unfold is_true.
+  rewrite N.eqb_eq.
+  unfold Unique.mkUniqueGrimily in *.
+  intuition congruence.
+Qed.
+
+
+Lemma In_varUnique_elem : forall a l, 
+    In (varUnique a) (map varUnique l) <-> 
+    Foldable.elem a l.
+Proof.
+  intros.
+  induction l.
+  - simpl. rewrite elem_nil.
+    split; intro. contradiction. discriminate.
+  - rewrite elem_cons.
+    unfold is_true.
+    rewrite orb_true_iff.
+    split.
+    intro h. inversion h.
+    left. 
+    rewrite <- varUnique_iff in *.
+    apply Eq_Symmetric in H.
+    auto.
+    right. tauto.
+    intro h.
+    rewrite <- IHl in h.
+    simpl.
+    destruct h.
+    left. 
+    rewrite <- varUnique_iff in *.
+    symmetry. auto.
+    right. auto.
+Qed.
+
+
+
 (** ** A DecidableType structure based on  [GHC.Base.==]. *)
 
 (* Define the Var type as a decidable type by using the Eq instance.
@@ -123,9 +137,9 @@ Qed.
 Module Var_as_DT <: BooleanDecidableType <: DecidableType.
   Definition t := Var.
 
-  Definition eqb : t -> t -> bool := _GHC.Base.==_.
+  Definition eqb : t -> t -> bool := _==_.
 
-  Definition eq : t -> t -> Prop := fun x y => eqb x y = true.
+  Definition eq : t -> t -> Prop := fun x y => eqb x y.
 
   Definition eq_equiv : Equivalence eq.
   Proof.
@@ -212,7 +226,7 @@ Qed.
 
 Lemma almostEqual_eq :
   forall v1 v2, 
-    almostEqual v1 v2 -> (v1 GHC.Base.== v2 = true).
+    almostEqual v1 v2 -> (v1 == v2).
 Proof.
   intros v1 v2 H.
   inversion H; unfold_zeze; simpl; apply N.eqb_refl.
