examples/ghc/theories/VarSet.v
@@ -1,49 +1,131 @@
+From Coq Require Import ssreflect ssrfun ssrbool.
+Require Import Psatz.
+Require Import Coq.Lists.List.
+Require Import Coq.NArith.BinNat.
+Import ListNotations.
+Require Import Coq.Classes.RelationClasses.
+Require Import Coq.Classes.Morphisms.
+Require Import SetoidList.
+
 Require Import GHC.Base.
+
+Require Import Proofs.GHC.Base.
+Require Import Proofs.GHC.List.
+Require Import Proofs.Data.Foldable.
+
 Require Import CoreFVs.
 Require Import Id.
 Require Import Core.
 Require UniqFM.
 
-Import GHC.Base.ManualNotations.
-
-Require Import Proofs.GHC.Base.
-Require Import Proofs.GHC.List.
-Require Import Proofs.Data.Foldable.
 Require Import Proofs.ContainerAxioms.
-
-Require Import Psatz.
-Require Import Coq.Lists.List.
-Require Import Coq.NArith.BinNat.
-
-Import ListNotations.
-
 Require Import Proofs.GhcTactics.
 Require Import Proofs.Unique.
 Require Import Proofs.Var.
-
-(* Require Import Proofs.ContainerAxioms.
-   Require Import IntSetProofs.  *)
-
 Require Import Proofs.VarSetFSet.
-
-
-Require Import Coq.Classes.RelationClasses.
-
 
 Open Scope Z_scope.
 
+
+Set Implicit Arguments.
+Unset Strict Implicit.
+Unset Printing Implicit Defensive.
 Set Bullet Behavior "Strict Subproofs".
 
-Ltac unfold_VarSet_to_IntMap :=
-  repeat match goal with
-         | [vs : VarSet |- _ ] =>
-           let u := fresh "u" in
-           destruct vs as [u]; destruct u; simpl
-         | [ |- UniqSet.Mk_UniqSet _ = UniqSet.Mk_UniqSet _ ] =>
-           f_equal
-         | [ |- UniqFM.UFM _ = UniqFM.UFM _ ] =>
-           f_equal
-         end.
+Ltac hs_simpl := autorewrite with hs_simpl.
+
+Tactic Notation "hs_simpl" "in" hyp(h) := autorewrite with hs_simpl in h.
+
+Lemma fold_is_true : forall b, b = true <-> is_true b.
+Proof. intros. unfold is_true. reflexivity. Qed.
+
+
+Axiom lookup_eq : forall A k k' (i : IntMap.Internal.IntMap A),
+    k == k'->
+    IntMap.Internal.lookup k i = IntMap.Internal.lookup k' i.
+
+Axiom delete_commute :
+  forall (A : Type)
+    (kx ky : Internal.Key) 
+    (i : Internal.IntMap A),
+  IntMap.Internal.delete ky (IntMap.Internal.delete kx i) =
+  IntMap.Internal.delete kx (IntMap.Internal.delete ky i).
+
+
+(* I would love to be able to use rewriting instead of this 
+   lemma to do this. Why doesn't it work??? *)
+Lemma eq_replace_r : forall a (v1 v2 v3 : a) `{EqLaws a}, 
+    (v2 == v3) -> (v1 == v2) = (v1 == v3).
+Proof.
+  intros.
+  rewrite -> H1. (* why does the ssreflect rewriting tactic not work here. *)
+  reflexivity.
+Qed.
+
+Lemma eq_replace_l : forall a (v1 v2 v3 : a) `{EqLaws a}, 
+    (v2 == v3) -> (v2 == v1) = (v3 == v1).
+Proof.
+  intros.
+  eapply Eq_m.
+  eauto.
+  eapply Eq_refl.
+Qed.
+
+
+(* Some cargo culting here. I'm not sure if we need to do all of this.*)
+
+Local Lemma parametric_eq_trans : forall (a : Type) (H : Eq_ a),
+  EqLaws a -> Transitive (fun x y : a => x == y).
+Proof.
+  intros.
+  intros x y z.
+  pose (k := Eq_trans).
+  eapply k.
+Defined. 
+
+Local Lemma parametric_eq_sym : forall (a : Type) (H : Eq_ a),
+  EqLaws a -> Symmetric (fun x y : a => x == y).
+Proof.
+  intros.
+  intros x y.
+  rewrite Eq_sym.
+  auto.
+Defined. 
+
+Add Parametric Relation {a}`{H: EqLaws a} : a 
+  (fun x y => x == y) 
+    reflexivity proved by Eq_refl 
+    symmetry proved by (@parametric_eq_sym a _ H)
+    transitivity proved by (@parametric_eq_trans a _ H) as parametric_eq.
+
+Instance: RewriteRelation (fun x y => x == y).
+
+
+Lemma eqlist_Foldable_elem : forall a (s s' : list a) `{EqLaws a}, 
+      eqlistA (fun x y => x == y) s s' ->
+      (forall a, Foldable.elem a s = Foldable.elem a s').
+Proof.
+  intros a s s' EQ EQL. intro H. induction H.
+  intro x.
+  rewrite elem_nil. auto.
+  intro y. 
+  repeat rewrite -> elem_cons.
+  rewrite IHeqlistA.
+  erewrite eq_replace_r; eauto.
+Qed.
+
+
+Lemma memE : forall (s : t) (x : elt), mem x s <-> In x s.
+Proof.
+  intros. unfold is_true. rewrite <- mem_iff. reflexivity. Qed.
+
+
+Lemma subsetE : forall (s s' : t), subset s s' <->  s [<=] s'.
+Proof.
+  intros. unfold is_true. rewrite <- subset_iff. reflexivity. Qed.
+
+
+
 
 (** ** Valid VarSets *)
 
@@ -51,7 +133,32 @@ Ltac unfold_VarSet_to_IntMap :=
    axiomatize it or add it to a sigma type in one of the definitions. *)
 
 Definition ValidVarSet (vs : VarSet) : Prop :=
-  forall v1 v2, lookupVarSet vs v1 = Some v2 -> (v1 GHC.Base.== v2) = true.
+  forall v1 v2, lookupVarSet vs v1 = Some v2 -> (v1 == v2).
+
+Axiom ValidVarSet_Axiom : forall vs, ValidVarSet vs.
+
+(** ** NOTE: VarSets and equality *)
+
+(* VarSets have several different notions of equality. 
+   In all three definitions, equal varsets must have the same domain. 
+   Now suppose:
+       lookupVarSet m1 x = Some v1 and
+       lookupVarSet m2 x = Some v2
+   The sets are equal when:
+    - v1 = v2                (i.e. coq equality) 
+    - almostEqual v1 v2      
+    - v1 == v2               (i.e. same uniques ONLY)
+
+   The last (coarsest) equality is the one used in the FSet signature, 
+   and denoted by the [=] notation. 
+
+   The almostEqual equality is denoted by {=}.
+
+   Because of this distinction, we have to do some lemmas twice: once 
+   for [=] equality, and once for {=} equality.
+  
+*)
+
 
 
 (** ** [VarSet] as FiniteSets  *)
@@ -83,9 +190,34 @@ Lemma minusVarSet_diff : forall x y, minusVarSet x y = diff x y.
 Lemma filterVarSet_filter : forall f x, filterVarSet f x = filter f x.
   reflexivity. Qed.
 
+
+(* This tactic rewrites the boolean functions into the 
+   set properties to make them more suitable for fsetdec. *)
+
+Ltac set_b_iff :=
+  repeat
+   progress
+    rewrite <- not_mem_iff in *
+  || rewrite <- mem_iff in *
+  || rewrite -> memE in *
+  || rewrite <- subset_iff in *
+  || rewrite -> subsetE in *
+  || rewrite <- is_empty_iff in *
+  || rewrite -> emptyVarSet_empty in *
+  || rewrite -> delVarSet_remove in *
+  || rewrite -> extendVarSet_add in *
+  || rewrite -> unionVarSet_union in *
+  || rewrite -> minusVarSet_diff in *
+  || rewrite -> filterVarSet_filter in *
+  || rewrite -> empty_b in *
+  || rewrite -> unitVarSet_singleton in *.
+
+
+
+(** List based operations in terms of folds *)
+
 Lemma extendVarSetList_foldl' : forall x xs, 
-    extendVarSetList x xs = 
-    Foldable.foldl' (fun x y => add y x) x xs.
+    extendVarSetList x xs = Foldable.foldl' (fun x y => add y x) x xs.
 Proof.
   intros.
   unfold extendVarSetList,
@@ -101,10 +233,7 @@ Lemma delVarSetList_foldl : forall vl vs,
 Proof. 
   induction vl.
   - intro vs. 
-    unfold delVarSetList.
-    unfold UniqSet.delListFromUniqSet.
-    destruct vs.
-    unfold UniqFM.delListFromUFM.
+    destruct vs. destruct getUniqSet'.
     unfold_Foldable_foldl.
     simpl.
     auto.
@@ -117,7 +246,7 @@ Proof.
     unfold_Foldable_foldl.
     simpl.
     intro IHvl.
-    rewrite IHvl with (vs:= (UniqSet.Mk_UniqSet (UniqFM.delFromUFM getUniqSet' a))).
+    rewrite (IHvl (UniqSet.Mk_UniqSet (UniqFM.delFromUFM getUniqSet' a))).
     auto.
 Qed.
 
@@ -128,32 +257,200 @@ Proof.
   reflexivity.
 Qed.
 
-Ltac rewrite_extendVarSetList := 
-  unfold extendVarSetList, UniqSet.addListToUniqSet;
-  replace UniqSet.addOneToUniqSet with (fun x y => add y x) by auto.
+Hint Rewrite mkVarSet_extendVarSetList : hs_simpl.
 
-(* This tactic rewrites the boolean functions into the 
-   set properties to make them more suitable for fsetdec. *)
 
-Ltac set_b_iff :=
-  repeat
-   progress
-    rewrite <- not_mem_iff in *
-  || rewrite <- mem_iff in *
-  || rewrite <- subset_iff in *
-  || rewrite <- is_empty_iff in *
-  || rewrite emptyVarSet_empty in *
-  || rewrite delVarSet_remove in *
-  || rewrite extendVarSet_add in *
-  || rewrite unionVarSet_union in *
-  || rewrite minusVarSet_diff in *
-  || rewrite filterVarSet_filter in *
-  || rewrite empty_b in *
-  || rewrite unitVarSet_singleton in *
-  || rewrite_extendVarSetList
-  || rewrite delVarSetList_foldl in *.
+(** ** [lookupVarSet] and [elemVarSet] correspondence *)
 
-(**************************************)
+Lemma lookupVarSet_elemVarSet : 
+  forall v1 v2 vs, lookupVarSet vs v1 = Some v2 -> elemVarSet v1 vs.
+Proof.
+  intros.
+  unfold lookupVarSet, elemVarSet in *.
+  unfold UniqSet.lookupUniqSet, UniqSet.elementOfUniqSet in *.
+  destruct vs.
+  unfold UniqFM.lookupUFM, UniqFM.elemUFM in *.
+  destruct getUniqSet'. 
+  set (key := Unique.getWordKey (Unique.getUnique v1)) in *.
+  rewrite member_lookup.
+  exists v2. auto.
+Qed.
+
+Lemma lookupVarSet_None_elemVarSet: 
+  forall v1 vs, lookupVarSet vs v1 = None <-> elemVarSet v1 vs = false.
+Proof.
+  intros.
+  unfold lookupVarSet, elemVarSet in *.
+  unfold UniqSet.lookupUniqSet, UniqSet.elementOfUniqSet in *.
+  destruct vs.
+  unfold UniqFM.lookupUFM, UniqFM.elemUFM in *.
+  destruct getUniqSet'.
+  set (key := Unique.getWordKey (Unique.getUnique v1)) in *.
+  rewrite non_member_lookup.
+  intuition.
+Qed.
+
+Lemma elemVarSet_lookupVarSet :
+  forall v1 vs, elemVarSet v1 vs -> exists v2, lookupVarSet vs v1 = Some v2.
+Proof.
+  intros.
+  unfold lookupVarSet, elemVarSet in *.
+  unfold UniqSet.lookupUniqSet, UniqSet.elementOfUniqSet in *.
+  destruct vs.
+  unfold UniqFM.lookupUFM, UniqFM.elemUFM in *.
+  destruct getUniqSet'.
+  set (key := Unique.getWordKey (Unique.getUnique v1)) in *.
+  rewrite <- member_lookup.
+  auto.
+Qed.
+
+(** ** [lookupVarSet] respects GHC.Base.== *)
+
+Lemma lookupVarSet_eq :
+  forall v1 v2 vs,
+    (v1 == v2) ->
+    lookupVarSet vs v1 = lookupVarSet vs v2.
+Proof. 
+  intros v1 v2 vs.
+  unfold lookupVarSet.
+  unfold UniqSet.lookupUniqSet.
+  destruct vs.
+  unfold UniqFM.lookupUFM.
+  destruct getUniqSet'.
+  intro h.
+  rewrite -> eq_unique in h.
+  rewrite h.
+  reflexivity.
+Qed.
+
+Ltac unfold_zeze_option := 
+    repeat unfold_zeze;
+           unfold Eq___option,
+           Base.Eq___option_op_zeze__.
+
+Instance lookupVarSet_m : 
+  Proper (Equal ==> (fun x y => x == y) ==> (fun x y => x == y)) lookupVarSet.
+Proof.
+  unfold Equal.
+  intros x y H v1 v2 EV.
+  erewrite lookupVarSet_eq; eauto.
+  pose (h1 := H v1).
+  pose (h2 := H v2).
+  repeat rewrite -> mem_iff in h1.
+  repeat rewrite -> mem_iff in h2.
+  destruct (lookupVarSet x v2) eqn:LX;
+  destruct (lookupVarSet y v2) eqn:LY;
+  unfold_zeze_option.
+  - apply ValidVarSet_Axiom in LX.
+    apply ValidVarSet_Axiom in LY.
+    eapply Eq_trans.
+    rewrite Eq_sym.
+    eapply LX.
+    eapply LY.
+  - apply lookupVarSet_elemVarSet in LX.
+    rewrite -> lookupVarSet_None_elemVarSet in LY.
+    set_b_iff.
+    intuition.
+  - apply lookupVarSet_elemVarSet in LY.
+    rewrite -> lookupVarSet_None_elemVarSet in LX.
+    set_b_iff.
+    intuition.
+  - auto.
+Qed.
+
+(** ** [elemVarSet] respects GHC.Base.== *)
+
+Lemma elemVarSet_eq : forall v1 v2 vs,
+  (v1 == v2) -> 
+  elemVarSet v1 vs = elemVarSet v2 vs.
+Proof.
+  intros v1 v2 vs h.
+  unfold elemVarSet, UniqSet.elementOfUniqSet.
+  destruct vs.
+  unfold UniqFM.elemUFM.
+  destruct getUniqSet'.
+  move: h.
+  rewrite eq_unique.
+  move=> h.
+  f_equal.
+  auto.
+Qed.
+
+
+(** ** [lookupVarSet . extendVarSet ] simplification *)
+
+Lemma lookupVarSet_extendVarSet_self:
+  forall v vs,
+  lookupVarSet (extendVarSet vs v) v = Some v.
+Proof.
+  intros.
+  unfold lookupVarSet, extendVarSet in *.
+  unfold UniqSet.lookupUniqSet, UniqSet.addOneToUniqSet in *.
+  destruct vs.
+  unfold UniqFM.lookupUFM, UniqFM.addToUFM in *.
+  destruct getUniqSet'.
+  set (key := Unique.getWordKey (Unique.getUnique v)) in *.
+  apply lookup_insert.
+Qed.
+
+Hint Rewrite lookupVarSet_extendVarSet_self : hs_simpl.
+
+Lemma lookupVarSet_extendVarSet_eq :
+      forall v1 v2 vs,
+      v1 == v2  ->
+      lookupVarSet (extendVarSet vs v1) v2 = Some v1.
+Proof.
+  intros v1 v2 vs H.
+  rewrite Eq_sym in H.
+  rewrite (lookupVarSet_eq _ H).
+  unfold lookupVarSet, extendVarSet.
+  unfold UniqSet.lookupUniqSet, UniqSet.addOneToUniqSet.
+  destruct vs.
+  unfold UniqFM.lookupUFM, UniqFM.addToUFM.
+  destruct getUniqSet'.
+  set (k1 := Unique.getWordKey (Unique.getUnique v1)).
+  rewrite lookup_insert.
+  reflexivity.
+Qed.
+
+Lemma lookupVarSet_extendVarSet_neq :
+      forall v1 v2 vs,
+      not (v1 == v2) ->
+      lookupVarSet (extendVarSet vs v1) v2 = lookupVarSet vs v2.
+Proof.
+  intros v1 v2 vs H.
+  assert (Unique.getWordKey (Unique.getUnique v1) <> 
+          Unique.getWordKey (Unique.getUnique v2)).
+  { intro h.
+    eapply H.
+    rewrite eq_unique.
+    auto.
+  }
+  unfold lookupVarSet, extendVarSet.
+  unfold UniqSet.lookupUniqSet, UniqSet.addOneToUniqSet.
+  destruct vs.
+  unfold UniqFM.lookupUFM, UniqFM.addToUFM.
+  destruct getUniqSet'.
+  eapply lookup_insert_neq.
+  auto.
+Qed.
+
+
+(* --------------------------------- *)
+
+(* Tactics that don't really work. *)
+                                   
+Local Ltac unfold_VarSet_to_IntMap :=
+  repeat match goal with
+         | [vs : VarSet |- _ ] =>
+           let u := fresh "u" in
+           destruct vs as [u]; destruct u; simpl
+         | [ |- UniqSet.Mk_UniqSet _ = UniqSet.Mk_UniqSet _ ] =>
+           f_equal
+         | [ |- UniqFM.UFM _ = UniqFM.UFM _ ] =>
+           f_equal
+         end.
+
 
 (* Q: is there a way to do the automatic destructs safely? Sometimes 
    loses too much information. *)
@@ -197,14 +494,13 @@ Ltac safe_unfold_VarSet :=
 
 (**************************************)
 
-(** ** [extendVarSetList]  *)
+(** ** [extendVarSetList] simplifications *)
 
 Lemma extendVarSetList_nil:
   forall s,
   extendVarSetList s [] = s.
 Proof.
   intro s.
-  set_b_iff.
   reflexivity.
 Qed.
 
@@ -213,8 +509,8 @@ Lemma extendVarSetList_cons:
   extendVarSetList s (v :: vs) = extendVarSetList (extendVarSet s v) vs.
 Proof.
   intros.
-  set_b_iff.
-  unfold_Foldable_foldl'.
+  rewrite extendVarSetList_foldl'.
+  autorewrite with hs_simpl.
   reflexivity.
 Qed.
 
@@ -228,58 +524,94 @@ Lemma extendVarSetList_append:
   extendVarSetList s (vs1 ++ vs2) = extendVarSetList (extendVarSetList s vs1) vs2.
 Proof.
   intros.
-  set_b_iff.
-  rewrite Foldable_foldl'_app.
-  auto.
+  rewrite extendVarSetList_foldl'.
+  autorewrite with hs_simpl.
+  reflexivity.
 Qed.
 
-(** ** [elemVarSet]  *)
+Hint Rewrite extendVarSetList_nil 
+             extendVarSetList_cons
+             extendVarSetList_singleton
+             extendVarSetList_append : hs_simpl.
 
-Lemma elemVarSet_emptyVarSet : forall v, elemVarSet v emptyVarSet = false.
+
+
+(** ** [delVarSetList] simplification  *)
+
+Lemma delVarSetList_nil:
+  forall e, delVarSetList e [] = e.
+Proof.
+  intros.
+  rewrite delVarSetList_foldl.
+  reflexivity.
+Qed.
+
+Lemma delVarSetList_single:
+  forall e a, delVarSetList e [a] = delVarSet e a.
+Proof.
+  intros.
+  rewrite delVarSetList_foldl.
+  autorewrite with hs_simpl.
+  reflexivity.
+Qed.
+
+Lemma delVarSetList_cons:
+  forall e a vs, delVarSetList e (a :: vs) = delVarSetList (delVarSet e a) vs.
+Proof.
+  intros.
+  repeat rewrite delVarSetList_foldl.
+  autorewrite with hs_simpl.
+  reflexivity.
+Qed.
+
+Lemma delVarSetList_app:
+  forall e vs vs', delVarSetList e (vs ++ vs') = delVarSetList (delVarSetList e vs) vs'.
+Proof.
+  intros.
+  repeat rewrite delVarSetList_foldl.
+  autorewrite with hs_simpl.
+  reflexivity.
+Qed.
+
+Hint Rewrite delVarSetList_nil 
+             delVarSetList_cons
+             delVarSetList_single
+             delVarSetList_app : hs_simpl.
+
+
+(** ** [elemVarSet] simplification *)
+
+Lemma elemVarSet_emptyVarSet : forall v, (elemVarSet v emptyVarSet) = false.
   intro v.
   set_b_iff.
   fsetdec.
 Qed.
 
-Lemma elemVarSet_unionVarSet:
-  forall v vs1 vs2,
-    elemVarSet v (unionVarSet vs1 vs2) =
-    elemVarSet v vs1 || elemVarSet v vs2.
+Lemma dbool : forall b, is_true b \/ not (is_true b).
 Proof.
-  intros.
-  set_b_iff.
-  destruct vs1 as [u].
-  destruct vs2 as [u0].
-  simpl.
-  unfold UniqFM.plusUFM.
-  destruct u.
-  destruct u0.
-  simpl.
-  symmetry.
-  destruct (IntMap.Internal.member
-              (realUnique v)
-              (IntMap.Internal.union i0 i)) eqn: Hu.
-  - rewrite member_lookup in Hu.
-    destruct Hu as [u Hu].
-    rewrite <- lookup_union in Hu.
-    apply orb_true_iff.
-    destruct Hu as [Hu | Hu].
-    + right.
-      rewrite member_lookup.
-      eauto.
-    +  destruct Hu as [? Hu].
-       left.
-       rewrite member_lookup.
-       eauto.
-  - rewrite non_member_lookup in Hu.
-    apply orb_false_iff.
-    split;
-      rewrite non_member_lookup;
-      rewrite <- lookup_union_None in Hu;
-      destruct Hu as [Hu1 Hu2];
-      assumption.
+  destruct b; auto.
 Qed.
 
+Axiom member_union :
+   forall (A : Type)
+     (key : Internal.Key) 
+     (i i0 : Internal.IntMap A),
+   (IntMap.Internal.member key (IntMap.Internal.union i i0)) = 
+   (IntMap.Internal.member key i0 || IntMap.Internal.member key i).
+
+
+Lemma elemVarSet_unionVarSet:
+  forall v vs1 vs2,
+    elemVarSet v (unionVarSet vs1 vs2) = elemVarSet v vs1 || elemVarSet v vs2.
+Proof.
+  move => v [[i]] [[i0]] /=.
+  rewrite member_union.
+  auto.
+Qed.
+
+Hint Rewrite elemVarSet_emptyVarSet elemVarSet_unionVarSet : hs_simpl.
+
+(*
 Lemma  In_hd_cons: forall v vs,
   In v (UniqSet.mkUniqSet (v :: vs)).
 Proof.
@@ -307,8 +639,7 @@ Proof.
   simpl.
   destruct (UniqSet.mkUniqSet (v :: vs)) as [u] eqn:Hus.
   destruct u.
-  
-Admitted.
+Abort.
   
 Lemma elemVarSet_cons_hd:
    forall v1 v2 vs, (v1 == v2) = true ->
@@ -324,8 +655,8 @@ Proof.
     assumption.
   - unfold mkVarSet.
     simpl.
-Admitted.
-  
+Abort.
+
   
 Lemma elemVarSet_cons: forall v1 v2 vs,
   (elemVarSet v1 (mkVarSet (v2 :: vs))) =
@@ -345,36 +676,9 @@ Proof.
     rewrite Heq.
     destruct (mkVarSet (v2 :: vs)) as [u] eqn:Hv.
     destruct u.
+Abort.
+*)
 
-    admit.
-  - admit.
-Admitted.
-  
-
-Lemma elemVarSet_extendVarSetList_r:
-  forall v s vs,
-  elemVarSet v (mkVarSet vs) = true ->
-  elemVarSet v (extendVarSetList s vs) = true.
-Proof.
-  intros.
-  induction vs.
-  - inversion H.
-  - rewrite elemVarSet_cons in H.
-    rewrite orb_true_iff in H.
-    destruct H as [H | H].
-    + clear IHvs. admit.
-    + 
-    revert H IHvs.
-    set_b_iff.
-    set (f:= fun x y => add y x).
-    intros H IHvs.
-    inversion H.
-    unfold In.
-    unfold elemVarSet, UniqSet.elementOfUniqSet.
-    unfold UniqFM.elemUFM.
-    simpl.    
-
-Admitted.
 
 
 (** ** [extendVarSet]  *)
@@ -382,17 +686,16 @@ Admitted.
 
 
 Lemma extendVarSet_elemVarSet_true : forall set v, 
-    elemVarSet v set = true -> extendVarSet set v [=] set.
+    elemVarSet v set -> extendVarSet set v [=] set.
 Proof. 
   intros.
   apply add_equal.
   auto.
 Qed.
 
-
 Lemma elemVarSet_extendVarSet:
   forall v vs v',
-  elemVarSet v (extendVarSet vs v') = (v' GHC.Base.== v) || elemVarSet v vs.
+  elemVarSet v (extendVarSet vs v') = (v' == v) || elemVarSet v vs.
 Proof.
   intros.
   unfold_zeze.
@@ -407,16 +710,397 @@ Proof.
     rewrite <- realUnique_eq in n; apply not_true_is_false in n; auto.
 Qed.
 
+Hint Rewrite elemVarSet_extendVarSet : hs_simpl.
+
+Lemma elemVarSet_extendVarSetList:
+  forall v vs vs',
+  elemVarSet v (extendVarSetList vs vs') = Foldable.elem v vs' || elemVarSet v vs.
+Proof.
+  intros.
+  generalize vs.
+  induction vs'.
+  + intros vs0. hs_simpl.
+    simpl.
+    auto.
+  + intros vs0. hs_simpl.
+    rewrite IHvs'.
+    hs_simpl.
+    rewrite elem_cons.
+    rewrite Eq_sym.
+    ssrbool.bool_congr.
+    reflexivity.
+Qed.
+
+Hint Rewrite elemVarSet_extendVarSetList : hs_simpl.
+
+Lemma extendVarSet_commute : forall x y vs, 
+    extendVarSet (extendVarSet vs y) x  [=] extendVarSet (extendVarSet vs x) y.
+Proof.
+  intros.
+  set_b_iff.
+  fsetdec.
+Qed.
+
+
+Lemma orE : forall a b, (a || b) <-> a \/ b.
+Proof. intros a b. unfold is_true. rewrite orb_true_iff. tauto. Qed.
+
+(** ** [extendVarSetList] **)
+
+(* These lemmas show that extendVarSetList respects [=] 
+    *)
+
+Lemma extendVarSetList_iff : forall l x vs,
+  In x (extendVarSetList vs l) <->
+  In x vs \/ Foldable.elem x l.
+Proof.
+  induction l.
+  - intros x vs.
+    hs_simpl.
+    rewrite elem_nil.
+    intuition.
+    inversion H0.
+  - intros x vs.
+    autorewrite with hs_simpl.
+    rewrite IHl.
+    rewrite elem_cons.
+    set_b_iff.
+    rewrite add_iff.
+    unfold Var_as_DT.eqb.
+    rewrite Eq_sym.
+    rewrite orE.
+    intuition.
+Qed.
+
+Lemma delVarSetList_iff : forall l x vs,
+  In x (delVarSetList vs l) <->
+  In x vs /\ ~ (Foldable.elem x l).
+Proof.
+  induction l.
+  - intros x vs. 
+    autorewrite with hs_simpl.
+    rewrite elem_nil.
+    intuition.
+  - intros x vs.
+    autorewrite with hs_simpl.
+    rewrite IHl.
+    rewrite elem_cons.
+    rewrite delVarSet_remove. rewrite remove_iff.
+    unfold Var_as_DT.eqb.
+    rewrite Eq_sym.
+    rewrite orE.
+    intuition.
+Qed.
+
+
+
+
+Instance extendVarSetList_m : 
+  Proper (Equal ==> (eqlistA (fun x y => x == y)) ==> Equal) extendVarSetList.
+Proof.
+  unfold Equal.
+  intros x y H s s' H0 a.
+  do 2 rewrite extendVarSetList_iff.
+  rewrite H.
+  intuition; right.
+  erewrite <- eqlist_Foldable_elem; eauto.
+  eapply EqLaws_Var.
+  erewrite eqlist_Foldable_elem; eauto.
+  eapply EqLaws_Var.
+Qed.
+
+Instance delVarSetList_m : 
+  Proper (Equal ==> (eqlistA (fun x y => x == y)) ==> Equal) delVarSetList.
+Proof.
+  unfold Equal.
+  intros x y H s s' H0 a.
+  do 2 rewrite delVarSetList_iff.
+  rewrite H.
+  intuition.
+  apply H3.
+  erewrite eqlist_Foldable_elem; eauto using EqLaws_Var.
+  apply H3.
+  erewrite <- eqlist_Foldable_elem; eauto using EqLaws_Var.
+Qed.
+
+
+(* We can commute the order of addition to varsets. 
+   This is only true for [=] *)
+Lemma extendVarSetList_extendVarSet_iff: forall l x vs,
+  extendVarSetList (extendVarSet vs x) l [=]
+  extendVarSet (extendVarSetList vs l) x.
+Proof.
+  induction l.
+  - intros.
+    hs_simpl.
+    reflexivity.
+  - intros.
+    hs_simpl.
+    rewrite extendVarSet_commute.
+    rewrite IHl.
+    reflexivity.
+Qed.
+
+
+Lemma elemVarSet_extend_add : forall v s vs a,
+  elemVarSet v (extendVarSetList s vs) ->
+  elemVarSet v (extendVarSetList (add a s) vs).
+Proof. 
+  intros v s vs a.
+  rewrite memE.
+  rewrite memE.
+  rewrite extendVarSetList_iff.
+  rewrite extendVarSetList_iff.
+  intuition.
+  left.
+  fsetdec.
+Qed.
+
+Lemma elemVarSet_extendVarSetList_r:
+  forall v s vs,
+  elemVarSet v (mkVarSet vs)  ->
+  elemVarSet v (extendVarSetList s vs) .
+Proof.
+  intros v s vs.
+  rewrite mkVarSet_extendVarSetList.
+  rewrite memE.
+  rewrite memE.
+  rewrite extendVarSetList_iff.
+  rewrite extendVarSetList_iff.
+  intuition.
+Qed.
+
 
 Lemma elemVarSet_mkVarSet_cons:
   forall v v' vs,
   elemVarSet v (mkVarSet (v' :: vs)) = false
   <-> (v' == v) = false /\ elemVarSet v (mkVarSet vs) = false.
 Proof.
-  intros.
-  rewrite !mkVarSet_extendVarSetList.
+  intros v v' vs.
+  rewrite mkVarSet_extendVarSetList.
   rewrite extendVarSetList_cons.
+  rewrite mkVarSet_extendVarSetList.
+  rewrite <- not_mem_iff.
+  rewrite <- not_mem_iff.
+  rewrite extendVarSetList_iff.
+  rewrite extendVarSetList_iff.
+  set_b_iff.
+  rewrite add_iff.
+  unfold Var_as_DT.eqb.
+  intuition.
+  apply not_true_is_false.
+  unfold not. auto.
+  destruct H.
+  rewrite H1 in H0.
+  done.
+Qed.
+
+(* We could axiomatize these in terms of In, but that would not be strong 
+   enough. As lookup is keyed on the uniques only, we need to specify 
+   list membership via Var's == only. *)
+
+Lemma lookupVarSet_extendVarSetList_false:
+  forall (vars:list Var) v vs,
+    not (Foldable.elem v vars ) -> 
+    lookupVarSet (extendVarSetList vs vars) v = lookupVarSet vs v.
+Proof.
+  elim=> v vs.
+  - rewrite elem_nil.
+    move => _.
+    hs_simpl.
+    done.
+  - move => IH v0 vs0.
+    hs_simpl.
+    rewrite elem_cons.
+    rewrite orE.
+    intuition.
+    rewrite IH.
+    rewrite lookupVarSet_extendVarSet_neq; try done.
+    intro h. apply H0. symmetry. done.
+    done.
+Qed.
+
+
+Ltac unfold_zeze :=
+  repeat unfold op_zeze__, op_zeze____, 
+  Eq___option, Base.Eq___option_op_zeze__,
+  Eq_Int___, 
+  Eq_Integer___, 
+  Eq_Word___, 
+  Eq_Char___, 
+  Eq_bool___, 
+  Eq_unit___ , 
+  Eq_comparison___, 
+  Eq_pair___ , 
+  Eq_list, 
+  Eq___NonEmpty, Base.Eq___NonEmpty_op_zeze__.
+
+
+Instance Foldable_proper : forall {a}`{EqLaws a},  
+  Proper ((fun (x y:a) => x == y) ==> (fun (x y:list a) => x == y) ==> Logic.eq)
+         Foldable.elem.
+Proof.
+  intros a E1 E2 x1 x2 Hx.
+  move => y1. induction y1.
+  - unfold_zeze. move => y2 Hy.
+    destruct y2.
+    auto.
+    simpl in Hy.
+    done.
+  - case;
+    unfold_zeze;
+    simpl.
+    done.
+    move => a1 l.
+    rewrite elem_cons.
+    rewrite elem_cons.
+    move/andP => [h0 h1].
+    rewrite (eq_replace_l a0 Hx).
+    rewrite (eq_replace_r x2 h0).
+    ssrbool.bool_congr.
+    eapply IHy1.
+    unfold_zeze.
+    auto.
+Qed.
+
+Lemma lookupVarSet_extendVarSetList_self:
+  forall (vars:list Var) v vs,
+    (Foldable.elem v vars) -> 
+    lookupVarSet (extendVarSetList vs vars) v == Some v.
+Proof.
+  induction vars.
+  - intros v vs H.
+    rewrite elem_nil in H.
+    done.
+  - intros v vs H.
+    rewrite elem_cons in H.
+    hs_simpl.
+    rewrite -> orE in H.
+    elim: H.
+    move => H.
+    case Hv: (Foldable.elem v vars).
+    + specialize (IHvars v (extendVarSet vs a)).
+      unfold is_true in *.
+      apply IHvars. 
+      done.
+    + rewrite (lookupVarSet_eq _ H).
+      rewrite lookupVarSet_extendVarSetList_false.
+      rewrite lookupVarSet_extendVarSet_self.
+      (** Still don't have a good way to simplify == *)
+      unfold op_zeze__, Eq___option, op_zeze____, Base.Eq___option_op_zeze__ .
+      symmetry. done.
+      intro h.
+      unfold is_true in h.
+      setoid_rewrite H in Hv.
+      rewrite Hv in h.
+      done.
+    + move=> h.
+      apply IHvars.
+      auto.
+Qed.
+
+Lemma lookupVarSet_extendVarSetList_l:
+  forall v vs1 vs2,
+  elemVarSet v (mkVarSet vs2) = false ->
+  lookupVarSet (extendVarSetList vs1 vs2) v = lookupVarSet vs1 v.
+Proof.
+  intros v vs1 vs2.
+  hs_simpl.
+  generalize emptyVarSet.
+  generalize vs1.
+  induction vs2.
+  - intros.  
+    hs_simpl.
+    auto.
+  - intros vs0 v0.
+    rewrite elem_cons. (* why does hs_simpl not do this?? *)
+    hs_simpl.
+    intro h.
+   
+    apply orb_false_elim in h.
+    destruct h as [h0 h3].
+    apply orb_false_elim in h0.
+    destruct h0 as [h1 h2].
+
+    rewrite lookupVarSet_extendVarSetList_false.
+    rewrite lookupVarSet_extendVarSet_neq.
+    reflexivity.
+
+    move => h4.
+    rewrite Eq_sym in h4.
+    rewrite h1 in h4.
+    done.
+
+    move => h4.
+    rewrite h2 in h4.
+    done. 
+Qed.
+    
+
+Lemma lookupVarSet_extendVarSetList_r_self:
+  forall v vs1 vs2,
+  List.In v vs2 ->
+  NoDup (map varUnique vs2) ->
+  lookupVarSet (extendVarSetList vs1 vs2) v = Some v.
+Proof.
+  move => v vs1 vs2.
+  move: vs1.
+  induction vs2; move=> vs1.
+  - move => IN.
+    inversion IN.
+  - move => IN ND.
+    simpl in ND.
+    inversion ND.
+    hs_simpl.
+    inversion IN; subst; hs_simpl; 
+      rewrite lookupVarSet_extendVarSetList_false; auto.
+    + rewrite lookupVarSet_extendVarSet_self.
+      auto.
+    + rewrite <- In_varUnique_elem.
+      auto.
+    + eapply in_map with (f:= varUnique) in H3.
+      assert (~ a == v).
+      { 
+        rewrite varUnique_iff.
+        move => h.
+        rewrite h in H1.
+        done.
+      }
 Admitted.
+
+
+(** ** [mkVarSet]  *)
+
+
+Lemma elemVarSet_mkVarset_iff_In:
+  forall v vs,
+  elemVarSet v (mkVarSet vs)  <->  List.In (varUnique v) (map varUnique vs).
+Proof.
+  intros.
+  rewrite mkVarSet_extendVarSetList.
+  induction vs.
+  - hs_simpl.
+    simpl.
+    done.
+  - hs_simpl.
+    simpl map.
+    split.
+    + rewrite orE => h.
+      destruct h as [h0|h1].
+      rewrite <- In_varUnique_elem in h0.
+      done.
+      done.
+    + move => h.
+      rewrite elem_cons. 
+      repeat rewrite orE. left.
+      inversion h.
+      ++ left.
+         rewrite varUnique_iff.
+         done.
+      ++ right.
+         rewrite -> In_varUnique_elem in H.
+         done.
+Qed.
 
 (** ** [delVarSet]  *)
 
@@ -444,60 +1128,103 @@ Lemma elemVarSet_delVarSet: forall v1 fvs v2,
   elemVarSet v1 (delVarSet fvs v2) = negb (v2 == v1) && elemVarSet v1 fvs.
 Proof.
   intros.
-  set_b_iff.
-Admitted.
+  destruct elemVarSet eqn:EL.
+  + symmetry.
+    apply andb_true_intro.
+    set_b_iff.
+    rewrite -> remove_iff in EL.
+    unfold Var_as_DT.eqb in EL. unfold not in EL.
+    rewrite negb_true_iff.
+    intuition.
+    apply not_true_is_false.
+    auto.
+  + symmetry.
+    apply not_true_is_false.
+    intro H.
+    apply andb_prop in H.
+    set_b_iff.
+    rewrite -> remove_iff in EL.
+    unfold Var_as_DT.eqb in *.
+    intuition.
+    rewrite -> negb_true_iff in H0.
+    apply H2.
+    intro h.
+    unfold Var_as_DT.t in *.
+    rewrite h in H0.
+    inversion H0.
+Qed.
+
+Lemma lookupVarSet_delVarSet_neq :
+      forall v1 v2 vs,
+      not (v1 == v2 ) ->
+      lookupVarSet (delVarSet vs v1) v2 = lookupVarSet vs v2.
+Proof.
+  intros v1 v2 vs H.
+  unfold lookupVarSet,delVarSet.
+  unfold UniqSet.lookupUniqSet, UniqSet.delOneFromUniqSet.
+  destruct vs.
+  unfold UniqFM.lookupUFM, UniqFM.delFromUFM.
+  destruct getUniqSet'.
+  assert (Unique.getWordKey (Unique.getUnique v1) <>
+          Unique.getWordKey (Unique.getUnique v2)).
+  { intro h. apply H. rewrite eq_unique. done. }
+  rewrite delete_neq.
+  auto.
+  auto.
+Qed.
 
 (** ** [delVarSetList]  *)
 
-Lemma delVarSetList_nil:
-  forall e, delVarSetList e [] = e.
+(* These next two rely on this strong property about the unique 
+   representations of IntMaps. *)
+Lemma delVarSet_commute : forall x y vs, 
+    delVarSet (delVarSet vs x) y = delVarSet (delVarSet vs y) x.
 Proof.
-  intros. unfold delVarSetList, delVarSet.
-  unfold UniqSet.delListFromUniqSet, UniqSet.delOneFromUniqSet.
-  destruct e; reflexivity.
-Qed.
-
-Lemma delVarSetList_single:
-  forall e a, delVarSetList e [a] = delVarSet e a.
-Proof.
-  intros. unfold delVarSetList, delVarSet.
-  unfold UniqSet.delListFromUniqSet, UniqSet.delOneFromUniqSet.
-  destruct e; reflexivity.
-Qed.
-
-Lemma delVarSetList_cons:
-  forall e a vs, delVarSetList e (a :: vs) = delVarSetList (delVarSet e a) vs.
-Proof.
-  induction vs; try revert IHvs;
-    unfold delVarSetList, UniqSet.delListFromUniqSet; destruct e;
-      try reflexivity.
+  intros.
+  unfold delVarSet.
+  unfold UniqSet.delOneFromUniqSet.
+  destruct vs.
+  f_equal.
+  unfold UniqFM.delFromUFM.
+  destruct getUniqSet'.
+  f_equal.
+  set (kx := Unique.getWordKey (Unique.getUnique x)).
+  set (ky := Unique.getWordKey (Unique.getUnique y)).
+  eapply delete_commute; eauto.
 Qed.
 
 Lemma delVarSetList_cons2:
-  forall e a vs, delVarSetList e (a :: vs) = delVarSet (delVarSetList e vs) a.
-Admitted.
-
-Lemma delVarSetList_app:
-  forall e vs vs', delVarSetList e (vs ++ vs') = delVarSetList (delVarSetList e vs) vs'.
+  forall vs e a, delVarSetList e (a :: vs) = delVarSet (delVarSetList e vs) a.
 Proof.
-  induction vs'.
-  - rewrite app_nil_r.
-    unfold delVarSetList, UniqSet.delListFromUniqSet.
-    destruct e; reflexivity.
-  - intros.
-    unfold delVarSetList, UniqSet.delListFromUniqSet; destruct e.
-    unfold UniqFM.delListFromUFM.
-Admitted.
-(*
-    repeat rewrite hs_coq_foldl_list. rewrite fold_left_app. reflexivity.
-Qed. *)
-
+  induction vs; intros e a1;
+  rewrite -> delVarSetList_cons in *.
+  - set_b_iff.
+    hs_simpl.
+    reflexivity.
+  - rewrite delVarSetList_cons.
+    rewrite delVarSetList_cons.
+    rewrite delVarSet_commute.
+    rewrite <- IHvs.
+    rewrite delVarSetList_cons.
+    auto.
+Qed.
 
 Lemma delVarSetList_rev:
   forall vs1 vs2,
   delVarSetList vs1 (rev vs2) = delVarSetList vs1 vs2.
-Admitted.
-
+Proof.
+  induction vs2.
+  - simpl. auto.
+  - simpl rev.
+    rewrite delVarSetList_cons.
+    rewrite delVarSetList_app.
+    rewrite IHvs2.
+    rewrite delVarSetList_cons.
+    rewrite delVarSetList_nil.
+    rewrite <- delVarSetList_cons2.
+    rewrite delVarSetList_cons.
+    reflexivity.
+Qed.
 
 Lemma elemVarSet_delVarSetList_false_l:
   forall v vs vs2,
@@ -513,11 +1240,29 @@ Proof.
     set_b_iff; fsetdec.
 Qed.
 
+Lemma delVarSet_unionVarSet:
+  forall vs1 vs2 x,
+  delVarSet (unionVarSet vs1 vs2) x [=] 
+  unionVarSet (delVarSet vs1 x) (delVarSet vs2 x).
+Proof.
+  intros.
+  set_b_iff.
+  fsetdec.
+Qed.
+
 Lemma delVarSetList_unionVarSet:
-  forall vs1 vs2 vs3,
+  forall vs3 vs1 vs2,
   delVarSetList (unionVarSet vs1 vs2) vs3 [=] 
   unionVarSet (delVarSetList vs1 vs3) (delVarSetList vs2 vs3).
-Admitted.
+Proof.
+  induction vs3; intros.
+  - repeat rewrite delVarSetList_nil.
+    reflexivity.
+  - repeat rewrite delVarSetList_cons.
+    rewrite delVarSet_unionVarSet.
+    rewrite IHvs3.
+    reflexivity.
+Qed.
 
 
 (**************************************)
@@ -527,7 +1272,7 @@ Admitted.
   
 Lemma subVarSet_refl:
   forall vs1,
-  subVarSet vs1 vs1 = true.
+  subVarSet vs1 vs1 .
 Proof.
   intros.
   set_b_iff.
@@ -536,9 +1281,9 @@ Qed.
 
 Lemma subVarSet_trans:
   forall vs1 vs2 vs3,
-  subVarSet vs1 vs2 = true ->
-  subVarSet vs2 vs3 = true ->
-  subVarSet vs1 vs3 = true.
+  subVarSet vs1 vs2  ->
+  subVarSet vs2 vs3  ->
+  subVarSet vs1 vs3 .
 Proof.
   intros.
   set_b_iff.
@@ -548,45 +1293,71 @@ Qed.
 
 Lemma subVarSet_emptyVarSet:
   forall vs,
-  subVarSet emptyVarSet vs = true.
+  subVarSet emptyVarSet vs .
 Proof.
   intros.
   set_b_iff.
   fsetdec.
 Qed.
 
+(*
 Lemma elemVarSet_unitVarSet: forall v1 v2,
-  (elemVarSet v1 (unitVarSet v2) = true) <-> (varUnique v1 = varUnique v2).
+  (elemVarSet v1 (unitVarSet v2) ) <-> (varUnique v1 = varUnique v2).
 Proof.
   intros v1 v2.
   set_b_iff.
   rewrite singleton_iff.
   unfold Var_as_DT.eqb.
   unfold_zeze.
-Admitted.
+Admitted. *)
+
+Lemma false_is_not_true :
+  forall b, b = false <-> b <> true.
+Proof.
+  destruct b; intuition.
+Qed.
 
 Lemma subVarSet_unitVarSet:
   forall v vs,
   subVarSet (unitVarSet v) vs = elemVarSet v vs.
-Admitted.
+Proof.
+  intros.
+  destruct subVarSet eqn:SV; symmetry.
+  + set_b_iff.
+    fsetdec.
+  + rewrite -> false_is_not_true in *.
+    set_b_iff.
+    intro h.
+    unfold Subset in SV.
+    apply SV.
+    intros.
+    rewrite In_eq_iff; eauto.
+Qed.
 
 Lemma elemVarSet_false_true:
   forall v1 fvs v2,
   elemVarSet v1 fvs = false ->
-  elemVarSet v2 fvs = true ->
+  elemVarSet v2 fvs  ->
   varUnique v1 <> varUnique v2.
 Proof.
   intros v1 fvs v2.
-  set_b_iff.
   intros.
-Admitted.
-  
+  assert (not (v2 == v1 )).
+  intro h. 
+  set_b_iff.
+  rewrite -> In_eq_iff in H0; eauto.
+  intro h.
+  rewrite <- varUnique_iff in h.
+  apply H1.
+  rewrite Eq_sym.
+  auto.
+Qed.
 
 Lemma subVarSet_elemVarSet_true:
   forall v vs vs',
-  subVarSet vs vs' = true ->
-  elemVarSet v vs = true ->
-  elemVarSet v vs' = true.
+  subVarSet vs vs'  ->
+  elemVarSet v vs  ->
+  elemVarSet v vs' .
 Proof.
   intros v vs vs'.
   set_b_iff.
@@ -595,7 +1366,7 @@ Qed.
 
 Lemma subVarSet_elemVarSet_false:
   forall v vs vs',
-  subVarSet vs vs' = true ->
+  subVarSet vs vs'  ->
   elemVarSet v vs' = false ->
   elemVarSet v vs = false.
 Proof.
@@ -606,8 +1377,8 @@ Qed.
 
 Lemma subVarSet_extendVarSetList_l:
   forall vs1 vs2 vs,
-  subVarSet vs1 vs2 = true ->
-  subVarSet vs1 (extendVarSetList vs2 vs) = true.
+  subVarSet vs1 vs2  ->
+  subVarSet vs1 (extendVarSetList vs2 vs) .
 Proof.
   intros vs1 vs2 vs.
   generalize vs2. clear vs2.
@@ -619,60 +1390,79 @@ Proof.
     set_b_iff. fsetdec.
 Qed.
 
-Lemma subVarSet_extendVarSetList_r:
-  forall vs vs1 vs2,
-  subVarSet vs1 (mkVarSet vs) = true ->
-  subVarSet vs1 (extendVarSetList vs2 vs) = true.
-Proof.
-  intros vs. 
-  induction vs; intros vs1 vs2.
-  - set_b_iff.
-    unfold_Foldable_foldl'.
-    simpl.
-    fsetdec.
-  - intro h. 
-    rewrite mkVarSet_extendVarSetList in h.
-    rewrite extendVarSetList_cons in *.
-Admitted.
-    
 
 
 Lemma subVarSet_extendVarSet_both:
   forall vs1 vs2 v,
-  subVarSet vs1 vs2 = true ->
-  subVarSet (extendVarSet vs1 v) (extendVarSet vs2 v) = true.
+  subVarSet vs1 vs2  ->
+  subVarSet (extendVarSet vs1 v) (extendVarSet vs2 v) .
 Proof.
   intros.
   set_b_iff.
   fsetdec.
 Qed.
+
 
 Lemma subVarSet_extendVarSet:
   forall vs1 vs2 v,
-  subVarSet vs1 vs2 = true ->
-  subVarSet vs1 (extendVarSet vs2 v) = true.
+  subVarSet vs1 vs2  ->
+  subVarSet vs1 (extendVarSet vs2 v) .
 Proof.
   intros.
   set_b_iff.
   fsetdec.
 Qed.
 
+
 Lemma subVarSet_extendVarSetList:
   forall vs1 vs2 vs3,
-  subVarSet vs1 vs2 = true ->
-  subVarSet vs1 (extendVarSetList vs2 vs3) = true.
-Admitted.
+  subVarSet vs1 vs2  ->
+  subVarSet vs1 (extendVarSetList vs2 vs3) .
+Proof.
+  induction vs3; autorewrite with hs_simpl.
+  - auto.
+  - intro h. 
+    rewrite extendVarSetList_extendVarSet_iff.
+    rewrite subVarSet_extendVarSet; auto.
+Qed.
 
 Lemma subVarSet_extendVarSet_l:
   forall vs1 vs2 v v',
-  subVarSet vs1 vs2 = true ->
+  subVarSet vs1 vs2  ->
   lookupVarSet vs2 v = Some v' ->
-  subVarSet (extendVarSet vs1 v) vs2 = true.
+  subVarSet (extendVarSet vs1 v) vs2 .
+Proof.
+  intros vs1 vs2 v v'.
+  intros s1 lu.
+  apply lookupVarSet_elemVarSet in lu.
+  set_b_iff.
+  rewrite <- (add_equal lu).
+  fsetdec.
+Qed.
+
+
+Lemma subVarSet_extendVarSetList_r:
+  forall vs vs1 vs2,
+  subVarSet vs1 (mkVarSet vs)  ->
+  subVarSet vs1 (extendVarSetList vs2 vs) .
+Proof.
+  intros vs. 
+  rewrite mkVarSet_extendVarSetList.
+  induction vs; intros vs1 vs2.
+  - autorewrite with hs_simpl.
+    set_b_iff.
+    fsetdec.
+  - intro h.     
+    autorewrite with hs_simpl in *.
+    rewrite -> extendVarSetList_extendVarSet_iff in *.
+    specialize (IHvs vs1 vs2).
+    set_b_iff.
 Admitted.
+    
 
 Lemma subVarSet_delVarSet:
   forall vs1 v,
-  subVarSet (delVarSet vs1 v) vs1 = true.
+  subVarSet (delVarSet vs1 v) vs1 .
 Proof.
   intros.
   set_b_iff.
@@ -682,19 +1472,18 @@ Qed.
 
 Lemma subVarSet_delVarSetList:
   forall vs1 vl,
-  subVarSet (delVarSetList vs1 vl) vs1 = true.
+  subVarSet (delVarSetList vs1 vl) vs1 .
 Proof.
   intros.
   set_b_iff.
   generalize vs1. clear vs1. induction vl.
-  - intros vs1. unfold_Foldable_foldl.
-    simpl.
+  - intros vs1. hs_simpl. 
     fsetdec.
   - intros vs1. revert IHvl.
-    unfold_Foldable_foldl.
+    hs_simpl.
     simpl.
     intro IH. 
-    rewrite IH with (vs1 := delVarSet vs1 a).
+    rewrite -> IH with (vs1 := delVarSet vs1 a).
     set_b_iff.
     fsetdec.
 Qed.
@@ -702,8 +1491,8 @@ Qed.
 
 Lemma subVarSet_delVarSetList_both:
   forall vs1 vs2 vl,
-  subVarSet vs1 vs2 = true ->
-  subVarSet (delVarSetList vs1 vl) (delVarSetList vs2 vl) = true.
+  subVarSet vs1 vs2  ->
+  subVarSet (delVarSetList vs1 vl) (delVarSetList vs2 vl) .
 Proof.
   intros.
   revert vs1 vs2 H. induction vl; intros.
@@ -717,8 +1506,8 @@ Qed.
 
 Lemma subVarSet_delVarSet_extendVarSet:
   forall jps isvs v,
-  subVarSet jps isvs = true ->
-  subVarSet (delVarSet jps v) (extendVarSet isvs v) = true.
+  subVarSet jps isvs  ->
+  subVarSet (delVarSet jps v) (extendVarSet isvs v) .
 Proof.
   intros.
   eapply subVarSet_trans.
@@ -729,8 +1518,8 @@ Qed.
 
 Lemma subVarSet_delVarSetList_extendVarSetList:
   forall jps isvs vs,
-  subVarSet jps isvs = true ->
-  subVarSet (delVarSetList jps vs) (extendVarSetList isvs vs) = true.
+  subVarSet jps isvs  ->
+  subVarSet (delVarSetList jps vs) (extendVarSetList isvs vs) .
 Proof.
   intros.
   eapply subVarSet_trans.
@@ -741,20 +1530,20 @@ Qed.
 
 Lemma subVarSet_delVarSetList_extendVarSetList_dual:
   forall jps isvs vs,
-  subVarSet jps (extendVarSetList isvs vs) = true ->
-  subVarSet (delVarSetList jps vs) isvs = true.
+  subVarSet jps (extendVarSetList isvs vs)  ->
+  subVarSet (delVarSetList jps vs) isvs .
 Admitted.
 
 Lemma mapUnionVarSet_In_subVarSet:
   forall a (x : a) xs f,
   List.In x xs ->
-  subVarSet (f x) (mapUnionVarSet f xs) = true.
+  subVarSet (f x) (mapUnionVarSet f xs) .
 Admitted.
 
 Lemma subVarSet_mapUnionVarSet:
   forall a (xs : list a) f vs,
-  Forall (fun x => subVarSet (f x) vs = true) xs ->
-  subVarSet (mapUnionVarSet f xs) vs = true.
+  Forall (fun x => subVarSet (f x) vs ) xs ->
+  subVarSet (mapUnionVarSet f xs) vs .
 Admitted.
 
 
@@ -769,24 +1558,6 @@ Proof.
 Admitted.
 
 
-(** ** [mkVarSet]  *)
-
-
-Lemma elemVarSet_mkVarset_iff_In:
-  forall v vs,
-  elemVarSet v (mkVarSet vs) = true <->  List.In (varUnique v) (map varUnique vs).
-Proof.
-  intros.
-  set_b_iff.
-  remember (mkVarSet vs) as vss.
-  unfold_VarSet.
-  rewrite <- getUnique_varUnique.
-  rewrite unique_In.
-  set (key := (Unique.getWordKey (Unique.getUnique v))).
-  (* Need theory about IntMap. *)
-Admitted. 
-
-
 
 
 (** ** [disjointVarSet]  *)
@@ -794,104 +1565,32 @@ Admitted.
 
 Axiom disjointVarSet_mkVarSet:
   forall vs1 vs2,
-  disjointVarSet vs1 (mkVarSet vs2) = true <->
+  disjointVarSet vs1 (mkVarSet vs2)  <->
   Forall (fun v => elemVarSet v vs1 = false) vs2.
 
 Axiom disjointVarSet_mkVarSet_nil:
   forall vs,
-  disjointVarSet vs (mkVarSet []) = true.
+  disjointVarSet vs (mkVarSet []) .
 
 
 Axiom disjointVarSet_mkVarSet_cons:
   forall v vs1 vs2,
-  disjointVarSet vs1 (mkVarSet (v :: vs2)) = true <->
-  elemVarSet v vs1 = false /\ disjointVarSet vs1 (mkVarSet vs2) = true.
+  disjointVarSet vs1 (mkVarSet (v :: vs2))  <->
+  elemVarSet v vs1 = false /\ disjointVarSet vs1 (mkVarSet vs2) .
 
 Axiom disjointVarSet_mkVarSet_append:
   forall vs1 vs2 vs3,
-  disjointVarSet vs1 (mkVarSet (vs2 ++ vs3)) = true <->
-  disjointVarSet vs1 (mkVarSet vs2) = true /\ disjointVarSet vs1 (mkVarSet vs3) = true.
+  disjointVarSet vs1 (mkVarSet (vs2 ++ vs3))  <->
+  disjointVarSet vs1 (mkVarSet vs2)  /\ disjointVarSet vs1 (mkVarSet vs3) .
 
 
 Axiom disjointVarSet_subVarSet_l:
   forall vs1 vs2 vs3,
-  disjointVarSet vs2 vs3 = true ->
-  subVarSet vs1 vs2 = true ->
-  disjointVarSet vs1 vs3 = true.
+  disjointVarSet vs2 vs3  ->
+  subVarSet vs1 vs2  ->
+  disjointVarSet vs1 vs3 .
 
 
-(** ** [lookupVarSet] *)
-
-Lemma lookupVarSet_elemVarSet : 
-  forall v1 v2 vs, lookupVarSet vs v1 = Some v2 -> elemVarSet v1 vs = true.
-Admitted.
-
-Lemma lookupVarSet_None_elemVarSet: 
-  forall v1 vs, lookupVarSet vs v1 = None <-> elemVarSet v1 vs = false.
-Admitted.
-
-Lemma elemVarSet_lookupVarSet :
-  forall v1 vs, elemVarSet v1 vs = true -> exists v2, lookupVarSet vs v1 = Some v2.
-Admitted.
-
-
-Lemma lookupVarSet_extendVarSet_self:
-  forall v vs,
-  lookupVarSet (extendVarSet vs v) v = Some v.
-Admitted.
-
-
-Lemma lookupVarSet_extendVarSetList_l:
-  forall v vs1 vs2,
-  elemVarSet v (mkVarSet vs2) = false ->
-  lookupVarSet (extendVarSetList vs1 vs2) v = lookupVarSet vs1 v.
-Admitted.
-
-Lemma lookupVarSet_extendVarSetList_r_self:
-  forall v vs1 vs2,
-  List.In v vs2 ->
-  NoDup (map varUnique vs2) ->
-  lookupVarSet (extendVarSetList vs1 vs2) v = Some v.
-Admitted.
-
-
-(** ** Compatibility with [GHC.Base.==] *)
-
-Lemma lookupVarSet_extendVarSet_eq :
-      forall v1 v2 vs,
-      v1 GHC.Base.== v2 = true ->
-      lookupVarSet (extendVarSet vs v1) v2 = Some v1.
-Proof.
-  intros.
-  unfold lookupVarSet, extendVarSet.
-  unfold UniqSet.lookupUniqSet, UniqSet.addOneToUniqSet.
-  destruct vs.
-  unfold UniqFM.lookupUFM, UniqFM.addToUFM.
-  destruct getUniqSet'.
-  unfold GHC.Base.op_zeze__, Eq___Var, Base.op_zeze____, 
-  Core.Eq___Var_op_zeze__ in H.
-Admitted.
-
-Axiom lookupVarSet_extendVarSet_neq :
-      forall v1 v2 vs,
-      not (v1 GHC.Base.== v2 = true) ->
-      lookupVarSet (extendVarSet vs v1) v2 = lookupVarSet vs v2.
-
-Axiom lookupVarSet_delVarSet_neq :
-      forall v1 v2 vs,
-      not (v1 GHC.Base.== v2 = true) ->
-      lookupVarSet (delVarSet vs v1) v2 = lookupVarSet vs v2.
-
-
-Axiom lookupVarSet_eq :
-  forall v1 v2 vs,
-    (v1 GHC.Base.== v2) = true ->
-    lookupVarSet vs v1 = lookupVarSet vs v2.
-
-Lemma elemVarSet_eq : forall v1 v2 vs,
-  (v1 GHC.Base.== v2) = true -> 
-  elemVarSet v1 vs = elemVarSet v2 vs.
-Admitted.
 
 
 (** ** [filterVarSet] *)
@@ -990,7 +1689,7 @@ Proof.
   unfold StrongSubset.
   intros var.
   destruct (var == v) eqn:EQV.
-  rewrite lookupVarSet_eq with (v2 := v); auto.
+  rewrite -> lookupVarSet_eq with (v2 := v); auto.
   rewrite H. auto.
   destruct (lookupVarSet vs var) eqn:Lvar; auto.
   rewrite lookupVarSet_extendVarSet_neq.
@@ -1001,7 +1700,7 @@ Qed.
 
 Lemma StrongSubset_extendList_fresh :
   forall vs vs2,
-  disjointVarSet vs (mkVarSet vs2) = true ->
+  disjointVarSet vs (mkVarSet vs2)  ->
   StrongSubset vs (extendVarSetList vs vs2).
 Proof.
   intros.
@@ -1128,9 +1827,8 @@ Proof.
   firstorder.
 Qed.
 
-
 Lemma Respects_StrongSubset_andb:
-  forall P Q,
+  forall (P Q : VarSet -> bool),
     Respects_StrongSubset (fun x => P x = true) ->
     Respects_StrongSubset (fun x => Q x = true) ->
     Respects_StrongSubset (fun x => P x && Q x = true).
@@ -1149,7 +1847,7 @@ Lemma Respects_StrongSubset_forall:
 Proof.
   unfold Respects_StrongSubset in *.
   intros.
-  rewrite Forall_forall in *.
+  rewrite -> Forall_forall in *.
   firstorder.
 Qed.
 
@@ -1160,8 +1858,8 @@ Lemma Respects_StrongSubset_forallb:
 Proof.
   unfold Respects_StrongSubset in *.
   intros.
-  rewrite forallb_forall in *.
-  rewrite Forall_forall in *.
+  rewrite -> forallb_forall in *.
+  rewrite -> Forall_forall in *.
   firstorder.
 Qed.
 
@@ -1210,10 +1908,10 @@ Lemma weaken:
 Proof. intros. unfold Respects_StrongSubset in R. eapply R; eassumption. Qed.
 
 Lemma weakenb:
-  forall {P : VarSet -> bool} {R : Respects_StrongSubset (fun x => P x = true)},
+  forall {P : VarSet -> bool} {R : Respects_StrongSubset (fun x => P x )},
   forall {vs1} {vs2},
   StrongSubset vs1 vs2 ->
-  P vs1 = true -> P vs2 = true.
+  P vs1  -> P vs2 .
 Proof. intros. unfold Respects_StrongSubset in R. eapply R; eassumption. Qed.
 
 Lemma Respects_StrongSubset_extendVarSet_ae:
@@ -1246,21 +1944,6 @@ Qed.
 
 
 
-(* We could axiomatize these in terms of In, but that would not be strong 
-   enough. As lookup is keyed on the uniques only, we need to specify 
-   list membership via Var's == only. *)
-
-Lemma lookupVarSet_extendVarSetList_self:
-  forall (vars:list Var) v vs,
-    Foldable.elem v vars = true -> 
-    lookupVarSet (extendVarSetList vs vars) v = Some v.
-Admitted.
-
-Lemma lookupVarSet_extendVarSetList_false:
-  forall (vars:list Var) v vs,
-    not (Foldable.elem v vars = true) -> 
-    lookupVarSet (extendVarSetList vs vars) v = lookupVarSet vs v.
-Admitted.
 
 
 (* A list of variables is fresh for a given varset when 
@@ -1270,7 +1953,7 @@ Admitted.
 *)
 
 Definition freshList (vars: list Var) (vs :VarSet) :=
-  (forall (v:Var), Foldable.elem v vars = true -> 
+  (forall (v:Var), Foldable.elem v vars  -> 
               lookupVarSet vs v = None).
 
 Lemma freshList_nil : forall v,  freshList nil v.
@@ -1286,7 +1969,7 @@ Proof.
   + intros [? ?] ? ?.
     rewrite elem_cons in H1.
     destruct (orb_prop _ _ H1) as [EQ|IN].
-    rewrite lookupVarSet_eq with (v2 := x); auto.
+    rewrite -> lookupVarSet_eq with (v2 := x); auto.
     eauto.
   + intros. split.
     eapply H. 
@@ -1351,7 +2034,7 @@ Admitted.
 
 Lemma StrongSubset_filterVarSet : 
   forall f1 f2 vs,
-  (forall v, f1 v = true -> f2 v = true) ->
+  (forall v, f1 v = true  -> f2 v = true) ->
   filterVarSet f1 vs {<=} filterVarSet f2 vs.
 Proof.  
 Admitted.
